theories/paris/examples/prf.v
@@ -1,0 +1,85 @@
+From clutch Require Import lib.flip.
+From clutch.paris Require Import paris map list.
+Set Default Proof Using "Type*".
+
+Section definition.
+
+  Variable Key Input Output : nat.
+
+  (* An idealised random function family. *)
+  Definition random_function : val :=
+    λ: "_key",
+      (* Create a reference to a functional map *)
+      let: "mapref" := init_map #() in
+      λ: "x",
+        match: get "mapref" "x" with
+        | SOME "y" => "y"
+        | NONE =>
+            let: "y" := (rand #Output) in
+            set "mapref" "x" "y";;
+            "y"
+        end.
+
+  Section spec.
+    Context `{!parisGS Σ}.
+
+    (* To hash a value v, we check whether it is in the map (i.e. it has been previously hashed).
+     If it has we return the saved hash value, otherwise we draw a hash value and save it in the map *)
+    Definition compute_rf_specialized hm : val :=
+      λ: "x",
+        match: get hm "x" with
+        | SOME "y" => "y"
+        | NONE =>
+            let: "y" := (rand #Output) in
+            set hm "x" "y";;
+            "y"
+        end.
+    Definition compute_rf : val :=
+      λ: "mapref" "x",
+        match: get "mapref" "x" with
+        | SOME "y" => "y"
+        | NONE =>
+            let: "y" := (rand #Output) in
+            set "mapref" "x" "y";;
+            "y"
+        end.
+
+    Definition is_random_function f m : iProp Σ :=
+      ∃ (mapref : loc), ⌜ f = compute_rf_specialized #mapref ⌝ ∗ map_list mapref ((λ b, LitV (LitInt b)) <$> m).
+
+    #[global] Instance timeless_is_random_function f m :
+      Timeless (is_random_function f m).
+    Proof. apply _. Qed.
+
+    Lemma wp_random_function E :
+      {{{ True }}}
+        random_function #() @ E
+        {{{ f, RET f; is_random_function f ∅ }}}.
+    Proof.
+      rewrite /random_function.
+      iIntros (Φ) "_ HΦ".
+      wp_pures.
+      wp_apply (wp_init_map with "[//]").
+      iIntros (?) "Hm". wp_pures.
+      iApply "HΦ". iExists _. rewrite fmap_empty. iFrame. eauto.
+    Qed.
+
+    Lemma wp_random_function_prev E f m (n : nat) (b : Z) :
+      m !! n = Some b →
+      {{{ is_random_function f m }}}
+        f #n @ E
+        {{{ RET #b; is_random_function f m }}}.
+    Proof.
+      iIntros (Hlookup Φ) "Hhash HΦ".
+      iDestruct "Hhash" as (hm ->) "H".
+      rewrite /compute_rf_specialized.
+      wp_pures.
+      wp_apply (wp_get with "[$]").
+      iIntros (vret) "(Hhash&->)".
+      rewrite lookup_fmap Hlookup /=. wp_pures. iModIntro. iApply "HΦ".
+      iExists _. eauto.
+    Qed.
+
+  End spec.
+
+End definition.
